cedar-lean/Cedar/Validation/RequestEntityValidator.lean
@@ -93,14 +93,19 @@ def instanceOfRequestType (request : Request) (reqty : RequestType) (schema: Ent
 
 /--
 For every entity in the store,
-1. The entity's type is defined in the type store.
+1. The entity's type is defined in the type store (either `ets` or `as` for action entities).
 2. The entity's attributes match the attribute types indicated in the type store.
 3. The entity's ancestors' types are consistent with the ancestor information
    in the type store.
 4. The entity's tags' types are consistent with the tags information in the type store.
+
+For every action in the entity store, the action's ancestors are consistent
+with the ancestor information in the action store.
 -/
-def instanceOfEntitySchema (entities : Entities) (ets : EntitySchema) (as : ActionSchema) : EntityValidationResult :=
-  entities.toList.forM λ (uid, data) => instanceOfEntityData uid data
+def instanceOfSchema (entities : Entities) (ets : EntitySchema) (as : ActionSchema) : EntityValidationResult :=
+  do
+    entities.toList.forM λ (uid, data) => instanceOfEntityData uid data
+    as.toList.forM λ (uid, data) => instanceOfActionSchemaData uid data
 where
   instanceOfEntityTags (data : EntityData) (entry : EntitySchemaEntry) : Bool :=
     match entry.tags? with
@@ -127,14 +132,6 @@ where
           else .error (.typeError s!"action entitiy {uid} cannot have tags")
         else .error (.typeError s!"action entitiy {uid} cannot have attributes")
       | _ => .error (.typeError "entity type not defined in type store")
-
-/--
-For every action in the entity store, the action's ancestors are consistent
-with the ancestor information in the action store.
--/
-def instanceOfActionSchema (entities : Entities) (as : ActionSchema) : EntityValidationResult :=
-  as.toList.forM λ (uid, data) => instanceOfActionSchemaData uid data
-where
   instanceOfActionSchemaData uid data :=
     match entities.find? uid with
       | .some entry => if data.ancestors == entry.ancestors
@@ -150,37 +147,13 @@ def validateRequest (schema : Schema) (request : Request) : RequestValidationRes
   else .error (.typeError "request could not be validated in any environment")
 
 def entitiesMatchEnvironment (env : Environment) (entities : Entities) : EntityValidationResult :=
-  instanceOfEntitySchema entities env.ets env.acts >>= λ _ => instanceOfActionSchema entities env.acts
+  instanceOfSchema entities env.ets env.acts
 
 def actionSchemaEntryToEntityData (ase : ActionSchemaEntry) : EntityData := {
   ancestors := ase.ancestors,
   attrs := Map.empty,
   tags := Map.empty
 }
-
-/--
-Update the entity schema with the entities created for action schema entries.
-This involves the construction of the ancestor information for the associated types
-by inspecting the concrete hierarchy.
--/
-def updateSchema (schema : Schema) (actionSchemaEntities : Entities) : Schema :=
-  let uniqueTys := Set.make (actionSchemaEntities.keys.map (·.ty)).elts
-  let newEntitySchemaEntries := uniqueTys.elts.map makeEntitySchemaEntries
-  {
-    ets := Map.make (schema.ets.kvs ++ newEntitySchemaEntries),
-    acts := schema.acts
-  }
-  where
-    makeEntitySchemaEntries ty :=
-      let entriesWithType := actionSchemaEntities.filter (λ k _ => k.ty == ty)
-      let allAncestorsForType := List.flatten (entriesWithType.values.map (λ edt =>
-        edt.ancestors.elts.map (·.ty) ))
-      let ese : EntitySchemaEntry := .standard {
-        ancestors := Set.make allAncestorsForType,
-        attrs := Map.empty,
-        tags := Option.none
-      }
-      (ty, ese)
 
 def validateEntities (schema : Schema) (entities : Entities) : EntityValidationResult :=
   schema.environments.forM (entitiesMatchEnvironment · entities)
